protocols/LabelsAlign.v
@@ -35,8 +35,8 @@ From KeyManagement Require Import
      AdversarySafety.
 
 From protocols Require Import
-     ExampleProtocols
-     ProtocolAutomation
+     (* ExampleProtocols *)
+     (* ProtocolAutomation *)
      ModelCheck
      SafeProtocol
      RealWorldStepLemmas
@@ -155,368 +155,7 @@ Proof.
     specialize (H3 _ _ H7); context_map_rewrites; eauto.
 Qed.
 
-Lemma step_reorder_no_recur :
-  forall A B C lbl1 suid1 uid1 (bd1 bd1' : data_step0 A B C),
-    step_user lbl1 suid1 bd1 bd1'
-    -> suid1 = Some uid1
-    -> forall D (bd2 bd2' : data_step0 A B D) lbl2 suid2 uid2,
-        step_user lbl2 suid2 bd2 bd2'
-        -> suid2 = Some uid2
-        -> uid1 <> uid2
-        -> forall cs cs1' cs2' (usrs usrs1' usrs2' : honest_users A) (adv adv1' adv2' : user_data B) gks gks1' gks2'
-            ks1 ks1' qmsgs1 qmsgs1' mycs1 mycs1' cmd1 cmd1' froms1 froms1' sents1 sents1' cur_n1 cur_n1'
-            ks2 ks2' qmsgs2 qmsgs2' mycs2 mycs2' cmd2 cmd2' froms2 froms2' sents2 sents2' cur_n2 cur_n2'
-            cmdc1 cmdc2,
-
-              bd1  = (usrs,   adv,   cs,   gks,   ks1,  qmsgs1,  mycs1,  froms1,  sents1,  cur_n1,  cmd1)
-            -> bd1' = (usrs1', adv1', cs1', gks1', ks1', qmsgs1', mycs1', froms1', sents1', cur_n1', cmd1')
-            -> bd2  = (usrs,   adv,   cs,   gks,   ks2,  qmsgs2,  mycs2,  froms2,  sents2,  cur_n2,  cmd2)
-            -> bd2' = (usrs2', adv2', cs2', gks2', ks2', qmsgs2', mycs2', froms2', sents2', cur_n2', cmd2')
-
-            -> nextAction cmd1 cmd1
-            -> nextAction cmd2 cmd2
-            -> nextAction cmdc2 cmd2
-            (* goodness *)
-            -> goodness_predicates (mkUniverse usrs adv cs gks)
-            -> syntactically_safe_U (mkUniverse usrs adv cs gks)
-            (* allow protocol to freely vary, since we won't be looking at it *)
-            -> usrs $? uid1 = Some (mkUserData ks1 cmdc1 qmsgs1 mycs1 froms1 sents1 cur_n1)
-            -> usrs $? uid2 = Some (mkUserData ks2 cmdc2 qmsgs2 mycs2 froms2 sents2 cur_n2)
-            -> forall cmdc1' usrs1'', 
-                usrs1'' = usrs1' $+ (uid1, mkUserData ks1' cmdc1' qmsgs1' mycs1' froms1' sents1' cur_n1')
-                -> usrs1'' $? uid2 = Some {| key_heap := ks2;
-                                            protocol := cmdc2;
-                                            msg_heap := qmsgs2;
-                                            c_heap := mycs2;
-                                            from_nons := froms2;
-                                            sent_nons := sents2;
-                                            cur_nonce := cur_n2 |}
-                -> exists bd2'',
-                  step_user lbl2 suid2
-                            (usrs1'', adv1', cs1', gks1', ks2, qmsgs2, mycs2, froms2, sents2, cur_n2, cmd2) bd2''.
-Proof.
-  (* destruct 1; destruct 2; inversion 3; inversion 1. why not this? too slow? *)
-  intros; cases cmd1; subst.
-  - cases cmd2; invert H1; invert H; clean_map_lookups; simpl.
-  - eapply nextAction_couldBe in H8. contradiction.
-  - cases cmd2; intros; invert H1; invert H; clean_map_lookups; simpl.
-    + eapply nextAction_couldBe in H9. contradiction.
-    + eapply nextAction_couldBe in H9. contradiction.
-    + econstructor; eauto. econstructor; eauto.
-    + destruct (uid ==n uid1); subst. econstructor; eauto. econstructor; eauto. congruence.
-      econstructor; eauto. econstructor; eauto. congruence.
-    + econstructor; eauto. econstructor; eauto.
-    + econstructor; eauto. econstructor; eauto.
-    + econstructor; eauto. econstructor; eauto.
-    + econstructor; eauto. econstructor; eauto.
-    + econstructor; eauto. econstructor; eauto.
-    + econstructor; eauto. econstructor; eauto.
-    + econstructor; eauto. econstructor; eauto.
-    + econstructor; eauto. econstructor; eauto.
-  - cases cmd2; intros; invert H1; invert H; clean_map_lookups; simpl.
-    + eapply nextAction_couldBe in H9. contradiction.
-    + eapply nextAction_couldBe in H9. contradiction.
-    + econstructor; eauto. econstructor; eauto.
-    + destruct (uid ==n uid1); subst; destruct (uid0 ==n uid1); subst.
-      * econstructor; eauto. econstructor; eauto.
-      * econstructor; eauto. econstructor; eauto.
-      * econstructor; eauto. econstructor; eauto. congruence.
-      * destruct (uid ==n uid0); subst. econstructor; eauto. econstructor; eauto. congruence.  
-        do 2 (econstructor; eauto). congruence.
-    + econstructor; eauto. econstructor; eauto.
-    + econstructor; eauto. econstructor; eauto.
-    + econstructor; eauto. econstructor; eauto.
-    + econstructor; eauto. econstructor; eauto.
-    + econstructor; eauto. econstructor; eauto.
-    + econstructor; eauto. econstructor; eauto.
-    + econstructor; eauto. econstructor; eauto.
-    + econstructor; eauto. econstructor; eauto.
-  - cases cmd2; invert H; invert H1; clean_map_lookups; simpl. (*; try (econstructor; eauto; econstructor; eauto).S*)
-    + eapply nextAction_couldBe in H9. contradiction.
-    + eapply nextAction_couldBe in H9. contradiction.
-    + eapply nextAction_couldBe in H9. contradiction.
-    + eapply nextAction_couldBe in H9. contradiction.
-    + econstructor; eauto. econstructor; eauto.
-    + econstructor; eauto. econstructor; eauto.
-    + destruct (uid ==n uid1); subst; econstructor; eauto; econstructor; eauto; congruence.
-    + destruct (uid ==n uid1); subst; econstructor; eauto; econstructor; eauto; congruence.
-    + econstructor; eauto. econstructor; eauto.
-    + econstructor; eauto. econstructor; eauto.
-    + econstructor; eauto. econstructor; eauto.
-    + econstructor; eauto. econstructor; eauto.
-    + econstructor; eauto. econstructor; eauto.
-    + econstructor; eauto. econstructor; eauto.
-    + econstructor; eauto. econstructor; eauto.
-    + econstructor; eauto. econstructor; eauto.
-    + econstructor; eauto. econstructor; eauto.
-    + econstructor; eauto. econstructor; eauto.
-    + econstructor; eauto. econstructor; eauto.
-    + econstructor; eauto. econstructor; eauto.
-    + econstructor; eauto. econstructor; eauto.
-    + econstructor; eauto. econstructor; eauto.
-    + econstructor; eauto. econstructor; eauto.
-    + econstructor; eauto. econstructor; eauto.
-  - cases cmd2; invert H; invert H1; clean_map_lookups; simpl.
-    + eapply nextAction_couldBe in H9. contradiction.
-    + eapply nextAction_couldBe in H9. contradiction.
-    + econstructor; eauto. econstructor.
-    + destruct (uid1 ==n uid). econstructor; eauto. econstructor; eauto.
-      intros. unfold syntactically_safe_U in H11. split_ex.
-      specialize (H12 uid2). simpl in *. generalize H14. intro H__new.
-      eapply H12 in H14. destruct H14. destruct H0 as [ H__syn H__typ ]. 
-      split_ex. (* is it possible to send to yourself? *)
-      simpl in *. unfold typingcontext_sound in *.
-      split_ex. specialize (H2 _ msg0 uid).
-      eapply syntactically_safe_na in H10; eauto. split_ex. invert H4. eapply H2 in H15.
-      split_ex. subst. destruct (c_id ==n x0); clean_map_lookups; eauto.
-      unfold keys_mine, findKeysCrypto in *. intros. clean_map_lookups. eapply H19 in H4.
-      eauto. eauto. congruence.
-
-      econstructor; eauto. econstructor; eauto.
-      intros. unfold syntactically_safe_U in H12. split_ex.
-      specialize (H12 uid2). simpl in *. generalize H14. intro H__newer.
-      eapply H12 in H__newer. destruct H__newer. destruct H0 as [ H__syn H__typ ]. 
-      split_ex. (* is it possible to send to yourself? *)
-      simpl in *. unfold typingcontext_sound in *.
-      split_ex. specialize (H2 _ msg0 uid).
-      eapply syntactically_safe_na in H10; eauto. split_ex. invert H4. eapply H2 in H16.
-      split_ex. subst. destruct (c_id ==n x0); clean_map_lookups; eauto.
-      unfold keys_mine, findKeysCrypto in *. intros. clean_map_lookups. eapply H20 in H4.
-      eauto. eauto. congruence.
-    + econstructor; eauto. econstructor; eauto.
-    + econstructor; eauto. econstructor; eauto.
-      unfold not in *. intros.  invert H.
-      * eapply H40. econstructor.
-      * eapply H40. econstructor; try eassumption. destruct (c_id0 ==n c_id); eauto.
-      * eapply H40. invert H6. econstructor; try eassumption.
-        destruct (c_id0 ==n c_id); subst; eauto.
-           unfold goodness_predicates in H11; split_ands. 
-           unfold message_queues_ok in H5. rewrite Forall_natmap_forall in H5. simpl in H5.
-           specialize (H5 _ _ H14). unfold message_queue_ok in H5; simpl in H5.
-           invert H5. split_ex. specialize (H15 _ eq_refl). tauto. eauto.
-    + econstructor; eauto.
-      eapply StepEncrypt with (c_id1 := next_key (cs $+ (c_id, SigEncCipher k__sign k__enc msg_to (Some uid1, cur_n1) msg))); eauto.
-      clean_map_lookups. eapply next_key_not_in. trivial.
-    + econstructor; eauto. econstructor; eauto.
-    + econstructor; eauto.
-      eapply StepSign with (c_id1 := next_key (cs $+ (c_id, SigEncCipher k__sign k__enc msg_to (Some uid1, cur_n1) msg))); eauto.
-      clean_map_lookups. eapply next_key_not_in. trivial.
-    + econstructor; eauto. econstructor; eauto.
-    + econstructor; eauto. econstructor; eauto.
-    + econstructor; eauto. econstructor; eauto.
-  - cases cmd2; invert H; invert H1; clean_map_lookups; simpl.
-    + eapply nextAction_couldBe in H9. contradiction.
-    + eapply nextAction_couldBe in H9. contradiction.
-    + econstructor; eauto. econstructor; eauto.
-    + destruct (uid ==n uid1); subst. econstructor; eauto. econstructor; eauto. congruence.
-      econstructor; eauto. econstructor; eauto. congruence. + econstructor; eauto. econstructor; eauto.
-    + econstructor; eauto. econstructor; eauto.
-    + econstructor; eauto. econstructor; eauto.
-    + econstructor; eauto. econstructor; eauto.
-    + econstructor; eauto. econstructor; eauto.
-    + econstructor; eauto. econstructor; eauto.
-    + econstructor; eauto. econstructor; eauto.
-    + econstructor; eauto. econstructor; eauto.
-  - cases cmd2; invert H; invert H1; clean_map_lookups; simpl.
-    + eapply nextAction_couldBe in H9. contradiction.
-    + eapply nextAction_couldBe in H9. contradiction.
-    + econstructor; eauto. econstructor; eauto.
-    + destruct (uid1 ==n uid). econstructor; eauto. econstructor; eauto.
-      intros. unfold syntactically_safe_U in H11. split_ex.
-      specialize (H12 uid2). simpl in *. generalize H14. intro H__new.
-      eapply H12 in H14. destruct H14. destruct H0 as [ H__syn H__typ ]. 
-      split_ex. (* is it possible to send to yourself? *)
-      simpl in *. unfold typingcontext_sound in *.
-      split_ex. specialize (H2 _ msg0 uid).
-      eapply syntactically_safe_na in H10; eauto. split_ex. invert H4. eapply H2 in H15.
-      split_ex. subst. destruct (c_id ==n x0); clean_map_lookups; eauto.
-      unfold keys_mine, findKeysCrypto in *. intros. clean_map_lookups. eapply H19 in H4.
-      eauto. eauto. congruence.
-
-      econstructor; eauto. econstructor; eauto.
-      intros. unfold syntactically_safe_U in H12. split_ex.
-      specialize (H12 uid2). simpl in *. generalize H14. intro H__newer.
-      eapply H12 in H__newer. destruct H__newer. destruct H0 as [ H__syn H__typ ]. 
-      split_ex. (* is it possible to send to yourself? *)
-      simpl in *. unfold typingcontext_sound in *.
-      split_ex. specialize (H2 _ msg0 uid).
-      eapply syntactically_safe_na in H10; eauto. split_ex. invert H4. eapply H2 in H16.
-      split_ex. subst. destruct (c_id ==n x0); clean_map_lookups; eauto.
-      unfold keys_mine, findKeysCrypto in *. intros. clean_map_lookups. eapply H20 in H4.
-      eauto. eauto. congruence.
-    + econstructor; eauto. econstructor; eauto.
-    + econstructor; eauto. econstructor; eauto.
-      unfold not in *. intros.  invert H.
-      * eapply H43. econstructor.
-      * eapply H43. invert H6. econstructor; try eassumption.
-        destruct (c_id0 ==n c_id); subst; eauto.
-           unfold goodness_predicates in H11; split_ands. 
-           unfold message_queues_ok in H5. rewrite Forall_natmap_forall in H5. simpl in H5.
-           specialize (H5 _ _ H14). unfold message_queue_ok in H5; simpl in H5.
-           invert H5. split_ex. specialize (H15 _ eq_refl). tauto. eauto.
-      * eapply H43. invert H6. econstructor; try eassumption.
-        destruct (c_id0 ==n c_id); subst; eauto.
-           unfold goodness_predicates in H11; split_ands. 
-           unfold message_queues_ok in H5. rewrite Forall_natmap_forall in H5.
-           specialize (H5 _ _ H14). unfold message_queue_ok in H5; simpl in H5.
-           invert H5. split_ex. specialize (H15 _ eq_refl). tauto.
-    + econstructor; eauto.  eapply StepEncrypt with (c_id1 := next_key (cs $+ (c_id, SigCipher k msg_to (Some uid1, cur_n1) msg))); eauto. clean_map_lookups. eapply next_key_not_in. trivial.
-    + econstructor; eauto. econstructor; eauto.
-    + econstructor; eauto.  eapply StepSign with (c_id1 := next_key (cs $+ (c_id, SigCipher k msg_to (Some uid1, cur_n1) msg))); eauto. clean_map_lookups. eapply next_key_not_in. trivial.
-    + econstructor; eauto. econstructor; eauto.
-    + econstructor; eauto. econstructor; eauto.
-    + econstructor; eauto. econstructor; eauto.
-  - cases cmd2; invert H; invert H1; clean_map_lookups; simpl.
-    + eapply nextAction_couldBe in H9. contradiction.
-    + eapply nextAction_couldBe in H9. contradiction.
-    + econstructor; eauto. econstructor; eauto.
-    + destruct (uid ==n uid1); subst. econstructor; eauto. econstructor; eauto. congruence.
-      econstructor; eauto. econstructor; eauto. congruence.
-    + econstructor; eauto. econstructor; eauto.
-    + econstructor; eauto. econstructor; eauto.
-    + econstructor; eauto. econstructor; eauto.
-    + econstructor; eauto. econstructor; eauto.
-    + econstructor; eauto. econstructor; eauto.
-    + econstructor; eauto. econstructor; eauto.
-    + econstructor; eauto. econstructor; eauto.
-    + econstructor; eauto. econstructor; eauto.
-  - cases cmd2; invert H; invert H1; clean_map_lookups; simpl.
-    + eapply nextAction_couldBe in H9. contradiction.
-    + eapply nextAction_couldBe in H9. contradiction.
-    + econstructor; eauto. econstructor; eauto.
-    + destruct (uid ==n uid1); subst. econstructor; eauto. econstructor; eauto. congruence.
-      econstructor; eauto. econstructor; eauto. congruence.
-    + econstructor; eauto. econstructor; eauto.
-    + econstructor; eauto. econstructor; eauto.
-    + econstructor; eauto. econstructor; eauto.
-    + econstructor; eauto. econstructor; eauto.
-    + econstructor; eauto. econstructor; eauto.
-    + econstructor; eauto. econstructor; eauto.
-    + econstructor; eauto. eapply StepGenerateSymKey with
-                               (k_id1 := next_key (gks $+ (k_id, {| keyId := k_id; keyUsage := usage; keyType := SymKey |}))); eauto.
-      eapply next_key_not_in. trivial.
-    + econstructor; eauto. eapply StepGenerateAsymKey with
-                               (k_id1 := next_key (gks $+ (k_id, {| keyId := k_id; keyUsage := usage; keyType := SymKey |}))); eauto.
-      eapply next_key_not_in. trivial.
-  - cases cmd2; invert H; invert H1; clean_map_lookups; simpl.
-    + eapply nextAction_couldBe in H9. contradiction.
-    + eapply nextAction_couldBe in H9. contradiction.
-    + econstructor; eauto. econstructor; eauto.
-    + destruct (uid ==n uid1); subst. econstructor; eauto. econstructor; eauto. congruence.
-      econstructor; eauto. econstructor; eauto. congruence.
-    + econstructor; eauto. econstructor; eauto.
-    + econstructor; eauto. econstructor; eauto.
-    + econstructor; eauto. econstructor; eauto.
-    + econstructor; eauto. econstructor; eauto.
-    + econstructor; eauto. econstructor; eauto.
-    + econstructor; eauto. econstructor; eauto.
-    + econstructor; eauto. eapply StepGenerateSymKey with (k_id1 := next_key (gks $+ (k_id, {| keyId := k_id; keyUsage := usage; keyType := AsymKey |}))); eauto.
-      eapply next_key_not_in. trivial.
-    + econstructor; eauto. eapply StepGenerateAsymKey with
-                              (k_id1 := next_key (gks $+ (k_id, {| keyId := k_id; keyUsage := usage; keyType := AsymKey |}))) ; eauto.
-      eapply next_key_not_in. trivial. Unshelve. eauto. eauto. eauto. eauto. eauto. eauto.
-      eauto. eauto. eauto. eauto.
-Qed.
-
-Hint Resolve step_reorder_no_recur.
-
-Lemma step_reorder_recur2 :
-  forall A B C lbl1 suid1 uid1 (bd1 bd1' : data_step0 A B C),
-    step_user lbl1 suid1 bd1 bd1'
-    -> suid1 = Some uid1
-    -> forall D (bd2 bd2' : data_step0 A B D) lbl2 suid2 uid2,
-        step_user lbl2 suid2 bd2 bd2'
-        -> suid2 = Some uid2
-        -> uid1 <> uid2
-        -> forall cs cs1' cs2' (usrs usrs1' usrs2' : honest_users A) (adv adv1' adv2' : user_data B) gks gks1' gks2'
-            ks1 ks1' qmsgs1 qmsgs1' mycs1 mycs1' cmd1 cmd1' froms1 froms1' sents1 sents1' cur_n1 cur_n1'
-            ks2 ks2' qmsgs2 qmsgs2' mycs2 mycs2' cmd2 cmd2' froms2 froms2' sents2 sents2' cur_n2 cur_n2'
-            cmdc1 cmdc2,
-
-              bd1  = (usrs,   adv,   cs,   gks,   ks1,  qmsgs1,  mycs1,  froms1,  sents1,  cur_n1,  cmd1)
-            -> bd1' = (usrs1', adv1', cs1', gks1', ks1', qmsgs1', mycs1', froms1', sents1', cur_n1', cmd1')
-            -> bd2  = (usrs,   adv,   cs,   gks,   ks2,  qmsgs2,  mycs2,  froms2,  sents2,  cur_n2,  cmd2)
-            -> bd2' = (usrs2', adv2', cs2', gks2', ks2', qmsgs2', mycs2', froms2', sents2', cur_n2', cmd2')
-
-            -> nextAction cmd1 cmd1
-            (* -> nextAction cmd2 cmd2 *)
-            -> nextAction cmdc2 cmd2
-            (* goodness *)
-            -> goodness_predicates (mkUniverse usrs adv cs gks)
-            -> syntactically_safe_U (mkUniverse usrs adv cs gks)
-            (* allow protocol to freely vary, since we won't be looking at it *)
-            -> usrs $? uid1 = Some (mkUserData ks1 cmdc1 qmsgs1 mycs1 froms1 sents1 cur_n1)
-            -> usrs $? uid2 = Some (mkUserData ks2 cmdc2 qmsgs2 mycs2 froms2 sents2 cur_n2)
-            -> forall cmdc1' usrs1'', 
-                usrs1'' = usrs1' $+ (uid1, mkUserData ks1' cmdc1' qmsgs1' mycs1' froms1' sents1' cur_n1')
-                -> usrs1'' $? uid2 = Some {| key_heap := ks2;
-                                            protocol := cmdc2;
-                                            msg_heap := qmsgs2;
-                                            c_heap := mycs2;
-                                            from_nons := froms2;
-                                            sent_nons := sents2;
-                                            cur_nonce := cur_n2 |}
-                -> exists bd2'',
-                  step_user lbl2 suid2
-                            (usrs1'', adv1', cs1', gks1', ks2, qmsgs2, mycs2, froms2, sents2, cur_n2, cmd2) bd2''.
-Proof.
-  intros; cases cmd1; subst.
-  - induction cmd2; invert H1; invert H; clean_map_lookups; simpl; eauto.
-  - admit.
-    (* induction cmd2; invert H1; invert H; clean_map_lookups; simpl.  *)
-  - induction cmd2; invert H1; invert H; clean_map_lookups; simpl; eauto.
-    + invert H9. admit.
-    + admit.
-    + invert H9. econstructor; eauto. econstructor; eauto. econstructor; eauto. econstructor; eauto.
-    + invert H9. destruct (uid ==n uid1); subst. econstructor; eauto. econstructor; eauto.
-      congruence. econstructor; eauto. econstructor; eauto. congruence. econstructor; eauto.
-      econstructor; eauto. 2: congruence. 
-      (* eassumption. econstructor; eauto. econstructor; eauto. *)
-Admitted.
-
-Lemma step_reorder_recur :
-  forall A B C lbl1 suid1 uid1 (bd1 bd1' : data_step0 A B C),
-    step_user lbl1 suid1 bd1 bd1'
-    -> suid1 = Some uid1
-    -> forall D (bd2 bd2' : data_step0 A B D) lbl2 suid2 uid2,
-        step_user lbl2 suid2 bd2 bd2'
-        -> suid2 = Some uid2
-        -> uid1 <> uid2
-        -> forall cs cs1' cs2' (usrs usrs1' usrs2' : honest_users A) (adv adv1' adv2' : user_data B) gks gks1' gks2'
-            ks1 ks1' qmsgs1 qmsgs1' mycs1 mycs1' cmd1 cmd1' froms1 froms1' sents1 sents1' cur_n1 cur_n1'
-            ks2 ks2' qmsgs2 qmsgs2' mycs2 mycs2' cmd2 cmd2' froms2 froms2' sents2 sents2' cur_n2 cur_n2'
-            cmdc1 cmdc2,
-
-              bd1  = (usrs,   adv,   cs,   gks,   ks1,  qmsgs1,  mycs1,  froms1,  sents1,  cur_n1,  cmd1)
-            -> bd1' = (usrs1', adv1', cs1', gks1', ks1', qmsgs1', mycs1', froms1', sents1', cur_n1', cmd1')
-            -> bd2  = (usrs,   adv,   cs,   gks,   ks2,  qmsgs2,  mycs2,  froms2,  sents2,  cur_n2,  cmd2)
-            -> bd2' = (usrs2', adv2', cs2', gks2', ks2', qmsgs2', mycs2', froms2', sents2', cur_n2', cmd2')
-
-            (* -> nextAction cmd1 cmd1 *)
-            (* -> nextAction cmd2 cmd2 *)
-            -> nextAction cmdc2 cmd2
-            (* goodness *)
-            -> goodness_predicates (mkUniverse usrs adv cs gks)
-            -> syntactically_safe_U (mkUniverse usrs adv cs gks)
-            (* allow protocol to freely vary, since we won't be looking at it *)
-            -> usrs $? uid1 = Some (mkUserData ks1 cmdc1 qmsgs1 mycs1 froms1 sents1 cur_n1)
-            -> usrs $? uid2 = Some (mkUserData ks2 cmdc2 qmsgs2 mycs2 froms2 sents2 cur_n2)
-            -> forall cmdc1' usrs1'', 
-                usrs1'' = usrs1' $+ (uid1, mkUserData ks1' cmdc1' qmsgs1' mycs1' froms1' sents1' cur_n1')
-                -> usrs1'' $? uid2 = Some {| key_heap := ks2;
-                                            protocol := cmdc2;
-                                            msg_heap := qmsgs2;
-                                            c_heap := mycs2;
-                                            from_nons := froms2;
-                                            sent_nons := sents2;
-                                            cur_nonce := cur_n2 |}
-                -> exists bd2'',
-                  step_user lbl2 suid2
-                            (usrs1'', adv1', cs1', gks1', ks2, qmsgs2, mycs2, froms2, sents2, cur_n2, cmd2) bd2''.
-Proof.
-Admitted.
-
-(* Lemma step_reorder : *)
+(* Lemma step_reorder_no_recur : *)
 (*   forall A B C lbl1 suid1 uid1 (bd1 bd1' : data_step0 A B C), *)
 (*     step_user lbl1 suid1 bd1 bd1' *)
 (*     -> suid1 = Some uid1 *)
@@ -534,40 +173,348 @@ Admitted.
 (*             -> bd2  = (usrs,   adv,   cs,   gks,   ks2,  qmsgs2,  mycs2,  froms2,  sents2,  cur_n2,  cmd2) *)
 (*             -> bd2' = (usrs2', adv2', cs2', gks2', ks2', qmsgs2', mycs2', froms2', sents2', cur_n2', cmd2') *)
 
+(*             -> nextAction cmd1 cmd1 *)
+(*             -> nextAction cmd2 cmd2 *)
+(*             -> nextAction cmdc2 cmd2 *)
+(*             (* goodness *) *)
+(*             -> goodness_predicates (mkUniverse usrs adv cs gks) *)
+(*             -> syntactically_safe_U (mkUniverse usrs adv cs gks) *)
 (*             (* allow protocol to freely vary, since we won't be looking at it *) *)
 (*             -> usrs $? uid1 = Some (mkUserData ks1 cmdc1 qmsgs1 mycs1 froms1 sents1 cur_n1) *)
 (*             -> usrs $? uid2 = Some (mkUserData ks2 cmdc2 qmsgs2 mycs2 froms2 sents2 cur_n2) *)
-(*             -> forall cmdc1' usrs1'' usr2', *)
+(*             -> forall cmdc1' usrs1'',  *)
 (*                 usrs1'' = usrs1' $+ (uid1, mkUserData ks1' cmdc1' qmsgs1' mycs1' froms1' sents1' cur_n1') *)
-(*                 -> usrs1'' $? uid2 = Some usr2' *)
+(*                 -> usrs1'' $? uid2 = Some {| key_heap := ks2; *)
+(*                                             protocol := cmdc2; *)
+(*                                             msg_heap := qmsgs2; *)
+(*                                             c_heap := mycs2; *)
+(*                                             from_nons := froms2; *)
+(*                                             sent_nons := sents2; *)
+(*                                             cur_nonce := cur_n2 |} *)
 (*                 -> exists bd2'', *)
 (*                   step_user lbl2 suid2 *)
-(*                             (build_data_step (mkUniverse usrs1'' adv1' cs1' gks1') usr2') bd2''. *)
+(*                             (usrs1'', adv1', cs1', gks1', ks2, qmsgs2, mycs2, froms2, sents2, cur_n2, cmd2) bd2''. *)
 (* Proof. *)
+(*   (* destruct 1; destruct 2; inversion 3; inversion 1. why not this? too slow? *) *)
+(*   intros; cases cmd1; subst. *)
+(*   - cases cmd2; invert H1; invert H; clean_map_lookups; simpl. *)
+(*   - eapply nextAction_couldBe in H8. contradiction. *)
+(*   - cases cmd2; intros; invert H1; invert H; clean_map_lookups; simpl. *)
+(*     + eapply nextAction_couldBe in H9. contradiction. *)
+(*     + eapply nextAction_couldBe in H9. contradiction. *)
+(*     + econstructor; eauto. econstructor; eauto. *)
+(*     + destruct (uid ==n uid1); subst. econstructor; eauto. econstructor; eauto. congruence. *)
+(*       econstructor; eauto. econstructor; eauto. congruence. *)
+(*     + econstructor; eauto. econstructor; eauto. *)
+(*     + econstructor; eauto. econstructor; eauto. *)
+(*     + econstructor; eauto. econstructor; eauto. *)
+(*     + econstructor; eauto. econstructor; eauto. *)
+(*     + econstructor; eauto. econstructor; eauto. *)
+(*     + econstructor; eauto. econstructor; eauto. *)
+(*     + econstructor; eauto. econstructor; eauto. *)
+(*     + econstructor; eauto. econstructor; eauto. *)
+(*   - cases cmd2; intros; invert H1; invert H; clean_map_lookups; simpl. *)
+(*     + eapply nextAction_couldBe in H9. contradiction. *)
+(*     + eapply nextAction_couldBe in H9. contradiction. *)
+(*     + econstructor; eauto. econstructor; eauto. *)
+(*     + destruct (uid ==n uid1); subst; destruct (uid0 ==n uid1); subst. *)
+(*       * econstructor; eauto. econstructor; eauto. *)
+(*       * econstructor; eauto. econstructor; eauto. *)
+(*       * econstructor; eauto. econstructor; eauto. congruence. *)
+(*       * destruct (uid ==n uid0); subst. econstructor; eauto. econstructor; eauto. congruence.   *)
+(*         do 2 (econstructor; eauto). congruence. *)
+(*     + econstructor; eauto. econstructor; eauto. *)
+(*     + econstructor; eauto. econstructor; eauto. *)
+(*     + econstructor; eauto. econstructor; eauto. *)
+(*     + econstructor; eauto. econstructor; eauto. *)
+(*     + econstructor; eauto. econstructor; eauto. *)
+(*     + econstructor; eauto. econstructor; eauto. *)
+(*     + econstructor; eauto. econstructor; eauto. *)
+(*     + econstructor; eauto. econstructor; eauto. *)
+(*   - cases cmd2; invert H; invert H1; clean_map_lookups; simpl. (*; try (econstructor; eauto; econstructor; eauto).S*) *)
+(*     + eapply nextAction_couldBe in H9. contradiction. *)
+(*     + eapply nextAction_couldBe in H9. contradiction. *)
+(*     + eapply nextAction_couldBe in H9. contradiction. *)
+(*     + eapply nextAction_couldBe in H9. contradiction. *)
+(*     + econstructor; eauto. econstructor; eauto. *)
+(*     + econstructor; eauto. econstructor; eauto. *)
+(*     + destruct (uid ==n uid1); subst; econstructor; eauto; econstructor; eauto; congruence. *)
+(*     + destruct (uid ==n uid1); subst; econstructor; eauto; econstructor; eauto; congruence. *)
+(*     + econstructor; eauto. econstructor; eauto. *)
+(*     + econstructor; eauto. econstructor; eauto. *)
+(*     + econstructor; eauto. econstructor; eauto. *)
+(*     + econstructor; eauto. econstructor; eauto. *)
+(*     + econstructor; eauto. econstructor; eauto. *)
+(*     + econstructor; eauto. econstructor; eauto. *)
+(*     + econstructor; eauto. econstructor; eauto. *)
+(*     + econstructor; eauto. econstructor; eauto. *)
+(*     + econstructor; eauto. econstructor; eauto. *)
+(*     + econstructor; eauto. econstructor; eauto. *)
+(*     + econstructor; eauto. econstructor; eauto. *)
+(*     + econstructor; eauto. econstructor; eauto. *)
+(*     + econstructor; eauto. econstructor; eauto. *)
+(*     + econstructor; eauto. econstructor; eauto. *)
+(*     + econstructor; eauto. econstructor; eauto. *)
+(*     + econstructor; eauto. econstructor; eauto. *)
+(*   - cases cmd2; invert H; invert H1; clean_map_lookups; simpl. *)
+(*     + eapply nextAction_couldBe in H9. contradiction. *)
+(*     + eapply nextAction_couldBe in H9. contradiction. *)
+(*     + econstructor; eauto. econstructor. *)
+(*     + destruct (uid1 ==n uid). econstructor; eauto. econstructor; eauto. *)
+(*       intros. unfold syntactically_safe_U in H11. split_ex. *)
+(*       specialize (H12 uid2). simpl in *. generalize H14. intro H__new. *)
+(*       eapply H12 in H14. destruct H14. destruct H0 as [ H__syn H__typ ].  *)
+(*       split_ex. (* is it possible to send to yourself? *) *)
+(*       simpl in *. unfold typingcontext_sound in *. *)
+(*       split_ex. specialize (H2 _ msg0 uid). *)
+(*       eapply syntactically_safe_na in H10; eauto. split_ex. invert H4. eapply H2 in H15. *)
+(*       split_ex. subst. destruct (c_id ==n x0); clean_map_lookups; eauto. *)
+(*       unfold keys_mine, findKeysCrypto in *. intros. clean_map_lookups. eapply H19 in H4. *)
+(*       eauto. eauto. congruence. *)
+
+(*       econstructor; eauto. econstructor; eauto. *)
+(*       intros. unfold syntactically_safe_U in H12. split_ex. *)
+(*       specialize (H12 uid2). simpl in *. generalize H14. intro H__newer. *)
+(*       eapply H12 in H__newer. destruct H__newer. destruct H0 as [ H__syn H__typ ].  *)
+(*       split_ex. (* is it possible to send to yourself? *) *)
+(*       simpl in *. unfold typingcontext_sound in *. *)
+(*       split_ex. specialize (H2 _ msg0 uid). *)
+(*       eapply syntactically_safe_na in H10; eauto. split_ex. invert H4. eapply H2 in H16. *)
+(*       split_ex. subst. destruct (c_id ==n x0); clean_map_lookups; eauto. *)
+(*       unfold keys_mine, findKeysCrypto in *. intros. clean_map_lookups. eapply H20 in H4. *)
+(*       eauto. eauto. congruence. *)
+(*     + econstructor; eauto. econstructor; eauto. *)
+(*     + econstructor; eauto. econstructor; eauto. *)
+(*       unfold not in *. intros.  invert H. *)
+(*       * eapply H40. econstructor. *)
+(*       * eapply H40. econstructor; try eassumption. destruct (c_id0 ==n c_id); eauto. *)
+(*       * eapply H40. invert H6. econstructor; try eassumption. *)
+(*         destruct (c_id0 ==n c_id); subst; eauto. *)
+(*            unfold goodness_predicates in H11; split_ands.  *)
+(*            unfold message_queues_ok in H5. rewrite Forall_natmap_forall in H5. simpl in H5. *)
+(*            specialize (H5 _ _ H14). unfold message_queue_ok in H5; simpl in H5. *)
+(*            invert H5. split_ex. specialize (H15 _ eq_refl). tauto. eauto. *)
+(*     + econstructor; eauto. *)
+(*       eapply StepEncrypt with (c_id1 := next_key (cs $+ (c_id, SigEncCipher k__sign k__enc msg_to (Some uid1, cur_n1) msg))); eauto. *)
+(*       clean_map_lookups. eapply next_key_not_in. trivial. *)
+(*     + econstructor; eauto. econstructor; eauto. *)
+(*     + econstructor; eauto. *)
+(*       eapply StepSign with (c_id1 := next_key (cs $+ (c_id, SigEncCipher k__sign k__enc msg_to (Some uid1, cur_n1) msg))); eauto. *)
+(*       clean_map_lookups. eapply next_key_not_in. trivial. *)
+(*     + econstructor; eauto. econstructor; eauto. *)
+(*     + econstructor; eauto. econstructor; eauto. *)
+(*     + econstructor; eauto. econstructor; eauto. *)
+(*   - cases cmd2; invert H; invert H1; clean_map_lookups; simpl. *)
+(*     + eapply nextAction_couldBe in H9. contradiction. *)
+(*     + eapply nextAction_couldBe in H9. contradiction. *)
+(*     + econstructor; eauto. econstructor; eauto. *)
+(*     + destruct (uid ==n uid1); subst. econstructor; eauto. econstructor; eauto. congruence. *)
+(*       econstructor; eauto. econstructor; eauto. congruence. + econstructor; eauto. econstructor; eauto. *)
+(*     + econstructor; eauto. econstructor; eauto. *)
+(*     + econstructor; eauto. econstructor; eauto. *)
+(*     + econstructor; eauto. econstructor; eauto. *)
+(*     + econstructor; eauto. econstructor; eauto. *)
+(*     + econstructor; eauto. econstructor; eauto. *)
+(*     + econstructor; eauto. econstructor; eauto. *)
+(*     + econstructor; eauto. econstructor; eauto. *)
+(*   - cases cmd2; invert H; invert H1; clean_map_lookups; simpl. *)
+(*     + eapply nextAction_couldBe in H9. contradiction. *)
+(*     + eapply nextAction_couldBe in H9. contradiction. *)
+(*     + econstructor; eauto. econstructor; eauto. *)
+(*     + destruct (uid1 ==n uid). econstructor; eauto. econstructor; eauto. *)
+(*       intros. unfold syntactically_safe_U in H11. split_ex. *)
+(*       specialize (H12 uid2). simpl in *. generalize H14. intro H__new. *)
+(*       eapply H12 in H14. destruct H14. destruct H0 as [ H__syn H__typ ].  *)
+(*       split_ex. (* is it possible to send to yourself? *) *)
+(*       simpl in *. unfold typingcontext_sound in *. *)
+(*       split_ex. specialize (H2 _ msg0 uid). *)
+(*       eapply syntactically_safe_na in H10; eauto. split_ex. invert H4. eapply H2 in H15. *)
+(*       split_ex. subst. destruct (c_id ==n x0); clean_map_lookups; eauto. *)
+(*       unfold keys_mine, findKeysCrypto in *. intros. clean_map_lookups. eapply H19 in H4. *)
+(*       eauto. eauto. congruence. *)
+
+(*       econstructor; eauto. econstructor; eauto. *)
+(*       intros. unfold syntactically_safe_U in H12. split_ex. *)
+(*       specialize (H12 uid2). simpl in *. generalize H14. intro H__newer. *)
+(*       eapply H12 in H__newer. destruct H__newer. destruct H0 as [ H__syn H__typ ].  *)
+(*       split_ex. (* is it possible to send to yourself? *) *)
+(*       simpl in *. unfold typingcontext_sound in *. *)
+(*       split_ex. specialize (H2 _ msg0 uid). *)
+(*       eapply syntactically_safe_na in H10; eauto. split_ex. invert H4. eapply H2 in H16. *)
+(*       split_ex. subst. destruct (c_id ==n x0); clean_map_lookups; eauto. *)
+(*       unfold keys_mine, findKeysCrypto in *. intros. clean_map_lookups. eapply H20 in H4. *)
+(*       eauto. eauto. congruence. *)
+(*     + econstructor; eauto. econstructor; eauto. *)
+(*     + econstructor; eauto. econstructor; eauto. *)
+(*       unfold not in *. intros.  invert H. *)
+(*       * eapply H43. econstructor. *)
+(*       * eapply H43. invert H6. econstructor; try eassumption. *)
+(*         destruct (c_id0 ==n c_id); subst; eauto. *)
+(*            unfold goodness_predicates in H11; split_ands.  *)
+(*            unfold message_queues_ok in H5. rewrite Forall_natmap_forall in H5. simpl in H5. *)
+(*            specialize (H5 _ _ H14). unfold message_queue_ok in H5; simpl in H5. *)
+(*            invert H5. split_ex. specialize (H15 _ eq_refl). tauto. eauto. *)
+(*       * eapply H43. invert H6. econstructor; try eassumption. *)
+(*         destruct (c_id0 ==n c_id); subst; eauto. *)
+(*            unfold goodness_predicates in H11; split_ands.  *)
+(*            unfold message_queues_ok in H5. rewrite Forall_natmap_forall in H5. *)
+(*            specialize (H5 _ _ H14). unfold message_queue_ok in H5; simpl in H5. *)
+(*            invert H5. split_ex. specialize (H15 _ eq_refl). tauto. *)
+(*     + econstructor; eauto.  eapply StepEncrypt with (c_id1 := next_key (cs $+ (c_id, SigCipher k msg_to (Some uid1, cur_n1) msg))); eauto. clean_map_lookups. eapply next_key_not_in. trivial. *)
+(*     + econstructor; eauto. econstructor; eauto. *)
+(*     + econstructor; eauto.  eapply StepSign with (c_id1 := next_key (cs $+ (c_id, SigCipher k msg_to (Some uid1, cur_n1) msg))); eauto. clean_map_lookups. eapply next_key_not_in. trivial. *)
+(*     + econstructor; eauto. econstructor; eauto. *)
+(*     + econstructor; eauto. econstructor; eauto. *)
+(*     + econstructor; eauto. econstructor; eauto. *)
+(*   - cases cmd2; invert H; invert H1; clean_map_lookups; simpl. *)
+(*     + eapply nextAction_couldBe in H9. contradiction. *)
+(*     + eapply nextAction_couldBe in H9. contradiction. *)
+(*     + econstructor; eauto. econstructor; eauto. *)
+(*     + destruct (uid ==n uid1); subst. econstructor; eauto. econstructor; eauto. congruence. *)
+(*       econstructor; eauto. econstructor; eauto. congruence. *)
+(*     + econstructor; eauto. econstructor; eauto. *)
+(*     + econstructor; eauto. econstructor; eauto. *)
+(*     + econstructor; eauto. econstructor; eauto. *)
+(*     + econstructor; eauto. econstructor; eauto. *)
+(*     + econstructor; eauto. econstructor; eauto. *)
+(*     + econstructor; eauto. econstructor; eauto. *)
+(*     + econstructor; eauto. econstructor; eauto. *)
+(*     + econstructor; eauto. econstructor; eauto. *)
+(*   - cases cmd2; invert H; invert H1; clean_map_lookups; simpl. *)
+(*     + eapply nextAction_couldBe in H9. contradiction. *)
+(*     + eapply nextAction_couldBe in H9. contradiction. *)
+(*     + econstructor; eauto. econstructor; eauto. *)
+(*     + destruct (uid ==n uid1); subst. econstructor; eauto. econstructor; eauto. congruence. *)
+(*       econstructor; eauto. econstructor; eauto. congruence. *)
+(*     + econstructor; eauto. econstructor; eauto. *)
+(*     + econstructor; eauto. econstructor; eauto. *)
+(*     + econstructor; eauto. econstructor; eauto. *)
+(*     + econstructor; eauto. econstructor; eauto. *)
+(*     + econstructor; eauto. econstructor; eauto. *)
+(*     + econstructor; eauto. econstructor; eauto. *)
+(*     + econstructor; eauto. eapply StepGenerateSymKey with *)
+(*                                (k_id1 := next_key (gks $+ (k_id, {| keyId := k_id; keyUsage := usage; keyType := SymKey |}))); eauto. *)
+(*       eapply next_key_not_in. trivial. *)
+(*     + econstructor; eauto. eapply StepGenerateAsymKey with *)
+(*                                (k_id1 := next_key (gks $+ (k_id, {| keyId := k_id; keyUsage := usage; keyType := SymKey |}))); eauto. *)
+(*       eapply next_key_not_in. trivial. *)
+(*   - cases cmd2; invert H; invert H1; clean_map_lookups; simpl. *)
+(*     + eapply nextAction_couldBe in H9. contradiction. *)
+(*     + eapply nextAction_couldBe in H9. contradiction. *)
+(*     + econstructor; eauto. econstructor; eauto. *)
+(*     + destruct (uid ==n uid1); subst. econstructor; eauto. econstructor; eauto. congruence. *)
+(*       econstructor; eauto. econstructor; eauto. congruence. *)
+(*     + econstructor; eauto. econstructor; eauto. *)
+(*     + econstructor; eauto. econstructor; eauto. *)
+(*     + econstructor; eauto. econstructor; eauto. *)
+(*     + econstructor; eauto. econstructor; eauto. *)
+(*     + econstructor; eauto. econstructor; eauto. *)
+(*     + econstructor; eauto. econstructor; eauto. *)
+(*     + econstructor; eauto. eapply StepGenerateSymKey with (k_id1 := next_key (gks $+ (k_id, {| keyId := k_id; keyUsage := usage; keyType := AsymKey |}))); eauto. *)
+(*       eapply next_key_not_in. trivial. *)
+(*     + econstructor; eauto. eapply StepGenerateAsymKey with *)
+(*                               (k_id1 := next_key (gks $+ (k_id, {| keyId := k_id; keyUsage := usage; keyType := AsymKey |}))) ; eauto. *)
+(*       eapply next_key_not_in. trivial. Unshelve. eauto. eauto. eauto. eauto. eauto. eauto. *)
+(*       eauto. eauto. eauto. eauto. *)
+(* Qed. *)
+
+(* Hint Resolve step_reorder_no_recur. *)
+
+(* Lemma step_reorder_recur2 : *)
+(*   forall A B C lbl1 suid1 uid1 (bd1 bd1' : data_step0 A B C), *)
+(*     step_user lbl1 suid1 bd1 bd1' *)
+(*     -> suid1 = Some uid1 *)
+(*     -> forall D (bd2 bd2' : data_step0 A B D) lbl2 suid2 uid2, *)
+(*         step_user lbl2 suid2 bd2 bd2' *)
+(*         -> suid2 = Some uid2 *)
+(*         -> uid1 <> uid2 *)
+(*         -> forall cs cs1' cs2' (usrs usrs1' usrs2' : honest_users A) (adv adv1' adv2' : user_data B) gks gks1' gks2' *)
+(*             ks1 ks1' qmsgs1 qmsgs1' mycs1 mycs1' cmd1 cmd1' froms1 froms1' sents1 sents1' cur_n1 cur_n1' *)
+(*             ks2 ks2' qmsgs2 qmsgs2' mycs2 mycs2' cmd2 cmd2' froms2 froms2' sents2 sents2' cur_n2 cur_n2' *)
+(*             cmdc1 cmdc2, *)
+
+(*               bd1  = (usrs,   adv,   cs,   gks,   ks1,  qmsgs1,  mycs1,  froms1,  sents1,  cur_n1,  cmd1) *)
+(*             -> bd1' = (usrs1', adv1', cs1', gks1', ks1', qmsgs1', mycs1', froms1', sents1', cur_n1', cmd1') *)
+(*             -> bd2  = (usrs,   adv,   cs,   gks,   ks2,  qmsgs2,  mycs2,  froms2,  sents2,  cur_n2,  cmd2) *)
+(*             -> bd2' = (usrs2', adv2', cs2', gks2', ks2', qmsgs2', mycs2', froms2', sents2', cur_n2', cmd2') *)
+
+(*             -> nextAction cmd1 cmd1 *)
+(*             (* -> nextAction cmd2 cmd2 *) *)
+(*             -> nextAction cmdc2 cmd2 *)
+(*             (* goodness *) *)
+(*             -> goodness_predicates (mkUniverse usrs adv cs gks) *)
+(*             -> syntactically_safe_U (mkUniverse usrs adv cs gks) *)
+(*             (* allow protocol to freely vary, since we won't be looking at it *) *)
+(*             -> usrs $? uid1 = Some (mkUserData ks1 cmdc1 qmsgs1 mycs1 froms1 sents1 cur_n1) *)
+(*             -> usrs $? uid2 = Some (mkUserData ks2 cmdc2 qmsgs2 mycs2 froms2 sents2 cur_n2) *)
+(*             -> forall cmdc1' usrs1'',  *)
+(*                 usrs1'' = usrs1' $+ (uid1, mkUserData ks1' cmdc1' qmsgs1' mycs1' froms1' sents1' cur_n1') *)
+(*                 -> usrs1'' $? uid2 = Some {| key_heap := ks2; *)
+(*                                             protocol := cmdc2; *)
+(*                                             msg_heap := qmsgs2; *)
+(*                                             c_heap := mycs2; *)
+(*                                             from_nons := froms2; *)
+(*                                             sent_nons := sents2; *)
+(*                                             cur_nonce := cur_n2 |} *)
+(*                 -> exists bd2'', *)
+(*                   step_user lbl2 suid2 *)
+(*                             (usrs1'', adv1', cs1', gks1', ks2, qmsgs2, mycs2, froms2, sents2, cur_n2, cmd2) bd2''. *)
+(* Proof. *)
+(*   intros; cases cmd1; subst. *)
+(*   - induction cmd2; invert H1; invert H; clean_map_lookups; simpl; eauto. *)
+(*   - admit. *)
+(*     (* induction cmd2; invert H1; invert H; clean_map_lookups; simpl.  *) *)
+(*   - induction cmd2; invert H1; invert H; clean_map_lookups; simpl; eauto. *)
+(*     + invert H9. admit. *)
+(*     + admit. *)
+(*     + invert H9. econstructor; eauto. econstructor; eauto. econstructor; eauto. econstructor; eauto. *)
+(*     + invert H9. destruct (uid ==n uid1); subst. econstructor; eauto. econstructor; eauto. *)
+(*       congruence. econstructor; eauto. econstructor; eauto. congruence. econstructor; eauto. *)
+(*       econstructor; eauto. 2: congruence.  *)
+(*       (* eassumption. econstructor; eauto. econstructor; eauto. *) *)
 (* Admitted. *)
 
-(* Lemma step_reorder_simple : *)
-(*   forall t__hon t__adv uid uid' u u' U bd' lbl1 lbl2 *)
-(*     (usrs : honest_users t__hon) (adv : user_data t__adv) cs gks ks qmsgs mycs froms sents cur_n cmd, *)
-    
-(*     step_user lbl1 (Some uid) (build_data_step  U u) (usrs,adv,cs,gks,ks,qmsgs,mycs,froms,sents,cur_n,cmd) *)
-(*     -> U.(users) $? uid = Some u *)
-(*     -> U.(users) $? uid' = Some u' *)
-(*     -> step_user lbl2 (Some uid') (build_data_step  U u') bd' *)
-(*     -> uid <> uid' *)
-(*     -> forall usrs' u'', usrs' = usrs $+ (uid, mkUserData ks cmd qmsgs mycs froms sents cur_n) *)
-(*     -> usrs' $? uid' = Some u'' *)
-(*     -> exists bd'', *)
-(*         step_user lbl2 (Some uid') *)
-(*                   (build_data_step (mkUniverse usrs' adv cs gks) u'') bd''. *)
+(* Lemma step_reorder_recur : *)
+(*   forall A B C lbl1 suid1 uid1 (bd1 bd1' : data_step0 A B C), *)
+(*     step_user lbl1 suid1 bd1 bd1' *)
+(*     -> suid1 = Some uid1 *)
+(*     -> forall D (bd2 bd2' : data_step0 A B D) lbl2 suid2 uid2, *)
+(*         step_user lbl2 suid2 bd2 bd2' *)
+(*         -> suid2 = Some uid2 *)
+(*         -> uid1 <> uid2 *)
+(*         -> forall cs cs1' cs2' (usrs usrs1' usrs2' : honest_users A) (adv adv1' adv2' : user_data B) gks gks1' gks2' *)
+(*             ks1 ks1' qmsgs1 qmsgs1' mycs1 mycs1' cmd1 cmd1' froms1 froms1' sents1 sents1' cur_n1 cur_n1' *)
+(*             ks2 ks2' qmsgs2 qmsgs2' mycs2 mycs2' cmd2 cmd2' froms2 froms2' sents2 sents2' cur_n2 cur_n2' *)
+(*             cmdc1 cmdc2, *)
+
+(*               bd1  = (usrs,   adv,   cs,   gks,   ks1,  qmsgs1,  mycs1,  froms1,  sents1,  cur_n1,  cmd1) *)
+(*             -> bd1' = (usrs1', adv1', cs1', gks1', ks1', qmsgs1', mycs1', froms1', sents1', cur_n1', cmd1') *)
+(*             -> bd2  = (usrs,   adv,   cs,   gks,   ks2,  qmsgs2,  mycs2,  froms2,  sents2,  cur_n2,  cmd2) *)
+(*             -> bd2' = (usrs2', adv2', cs2', gks2', ks2', qmsgs2', mycs2', froms2', sents2', cur_n2', cmd2') *)
+
+(*             (* -> nextAction cmd1 cmd1 *) *)
+(*             (* -> nextAction cmd2 cmd2 *) *)
+(*             -> nextAction cmdc2 cmd2 *)
+(*             (* goodness *) *)
+(*             -> goodness_predicates (mkUniverse usrs adv cs gks) *)
+(*             -> syntactically_safe_U (mkUniverse usrs adv cs gks) *)
+(*             (* allow protocol to freely vary, since we won't be looking at it *) *)
+(*             -> usrs $? uid1 = Some (mkUserData ks1 cmdc1 qmsgs1 mycs1 froms1 sents1 cur_n1) *)
+(*             -> usrs $? uid2 = Some (mkUserData ks2 cmdc2 qmsgs2 mycs2 froms2 sents2 cur_n2) *)
+(*             -> forall cmdc1' usrs1'',  *)
+(*                 usrs1'' = usrs1' $+ (uid1, mkUserData ks1' cmdc1' qmsgs1' mycs1' froms1' sents1' cur_n1') *)
+(*                 -> usrs1'' $? uid2 = Some {| key_heap := ks2; *)
+(*                                             protocol := cmdc2; *)
+(*                                             msg_heap := qmsgs2; *)
+(*                                             c_heap := mycs2; *)
+(*                                             from_nons := froms2; *)
+(*                                             sent_nons := sents2; *)
+(*                                             cur_nonce := cur_n2 |} *)
+(*                 -> exists bd2'', *)
+(*                   step_user lbl2 suid2 *)
+(*                             (usrs1'', adv1', cs1', gks1', ks2, qmsgs2, mycs2, froms2, sents2, cur_n2, cmd2) bd2''. *)
 (* Proof. *)
-(*   intros; *)
-(*     destruct U, u, u'; *)
-(*     dt bd'; *)
-(*     unfold build_data_step in *; *)
-(*     simpl in *; *)
-(*     eapply step_reorder with (suid1 := Some uid) (suid2 := Some uid'); eauto. *)
-(* Qed. *)
+(* Admitted. *)
 
 Lemma labels_align_user_step :
     forall {A B} suid (bd bd' : data_step0 A B (Base A)),
@@ -648,9 +595,8 @@ Proof.
   destruct st as [[ru iu] v].
   destruct st' as [[ru' iu'] v'].
   split_ex; subst.
-  invert H; eauto.
-  simpl in H0; 
-    invert H5; dismiss_adv.
+  invert H; simpl in *; try discriminate; eauto.
+  invert H6; dismiss_adv.
   split; trivial.
   
   destruct ru, userData; simpl in *.
