protocols/ShareSecretProtocol3.v
@@ -33,7 +33,8 @@ Require Import
         UniverseEqAutomation
         ProtocolAutomation
         SafeProtocol
-        ProtocolFunctions.
+        ProtocolFunctions
+        PartialOrderReduction.
 
 Require IdealWorld RealWorld.
 
@@ -153,14 +154,256 @@ Module ShareSecretProtocolSecure <: AutomatedSafeProtocol.
        mkKeys
     : core.
 
+  (* Section Summary. *)
+  (*   Import RealWorld. *)
+
+  (*   Ltac build_summary proto s := *)
+  (*     match proto with *)
+  (*     | Send ?uid _ => constr:({| sending_to := s.(sending_to) \cup { uid } |}) *)
+  (*     | Bind ?cmd1 ?cmd2 => *)
+  (*       let s1 := build_summary cmd1 s *)
+  (*       in  build_summary (cmd2 ?v) s1 *)
+  (*     | _ => s *)
+  (*     end. *)
+
+  (*   Check build_summary (@Return (Base Nat) 1) {| sending_to := { } |}. *)
+      
+
+  (*   Fixpoint build_summary {t} (proto : RealWorld.user_cmd t) (s : summary ) : summary := *)
+  (*     match proto with *)
+  (*     | Send uid m => {| sending_to := s.(sending_to) \cup { uid } |} *)
+  (*     | Bind cmd1 cmd2 => *)
+  (*       let s1 := build_summary cmd1 *)
+  (*       in  let s2 := build_summary (cmd2 v) *)
+  (*           in   *)
+  (*     | _ => s *)
+  (*     end. *)
+
+
+  (* Record summary := { sending_to : Sets.set user_id }. *)
+
+  (* Inductive summarize : forall {t}, user_cmd t -> summary -> Prop := *)
+  (* | SumReturn : forall t r s, *)
+  (*     summarize (@Return t r) s *)
+  (* | SumGen : forall s, *)
+  (*     summarize Gen s *)
+  (* | SumSend : forall {t} (msg : crypto t) uid s, *)
+  (*     Sets.In uid s.(sending_to) *)
+  (*     -> summarize (Send uid msg) s *)
+  (* | SumRecv : forall t pat s, *)
+  (*     summarize (@Recv t pat) s *)
+  (* | SumSignEncrypt : forall t k__s k__e u_id (msg : message t)s , *)
+  (*     summarize (SignEncrypt k__s k__e u_id msg) s *)
+  (* | SumDecrypt : forall t (msg : crypto t) s, *)
+  (*     summarize (Decrypt msg) s *)
+  (* | SumSign : forall t k u_id (msg : message t) s, *)
+  (*     summarize (Sign k u_id msg) s *)
+  (* | SumVerify : forall t k (msg : crypto t) s, *)
+  (*     summarize (Verify k msg) s *)
+  (* | SumGenSymKey : forall usg s, *)
+  (*     summarize (GenerateSymKey usg) s *)
+  (* | SumGenAsymKey : forall usg s, *)
+  (*     summarize (GenerateAsymKey usg) s *)
+  (* | SumBind : forall t1 t2 (c1 : user_cmd t1) (c2 : << t1 >> -> user_cmd t2) s, *)
+  (*     summarize c1 s *)
+  (*     -> (forall r__v, summarize (c2 r__v) s) *)
+  (*     -> summarize (Bind c1 c2) s *)
+  (* . *)
+  
+  Ltac build_summary proto s :=
+    match proto with
+    | RealWorld.Send ?uid _ =>
+      let s1 := constr:({| sending_to := s.(sending_to) \cup { uid } |}) in eval simpl in s1
+    | RealWorld.Bind ?cmd1 ?cmd2 =>
+      match cmd2 with
+      | (fun v:?V => ?CMD) =>
+        let s1 := build_summary cmd1 s
+        in  let s2 := build_summary CMD s1
+            in eval simpl in s2
+      (* | _ => *)
+      (*   constr:({| sending_to := s.(sending_to) \cup { 2000 } |}) *)
+      end
+    | _ => s
+    end.
+
+  (* Import RealWorld. *)
+  (* Import RealWorld.RealWorldNotations. *)
+
+
+
+  (* let s := build_summary (@Return (Base Nat) 1) constr:({| sending_to := { } |}) *)
+  (* in  idtac s. *)
+
+  (* let s := build_summary ( Send 0 (Content (message.Content 100)) ) *)
+  (*                        constr:({| sending_to := { } |}) *)
+  (* in  idtac s. *)
+  
+
+  (* let s := build_summary ( _ <- Send 0 (Content (message.Content 100)); @Return (Base Unit) tt) *)
+  (*                        constr:({| sending_to := { } |}) *)
+  (* in  idtac s. *)
+
+
+  (* Lemma build_summary_summarizes : *)
+  (*   forall t (proto : RealWorld.user_cmd t) s, *)
+  (*     s = build_summary proto {| sending_to := { } |} *)
+  (*     -> summarize proto s. *)
+      
+  
   Lemma safe_invariant :
     invariantFor
-      {| Initial := {(ru0, iu0, true)}; Step := @step t__hon t__adv  |}
+      {| Initial := {(ru0, iu0, true)}; Step := @stepC t__hon t__adv  |}
       (fun st => safety st /\ alignment st ).
   Proof.
     eapply invariant_weaken.
 
     - eapply multiStepClosure_ok; simpl.
+
+      eapply MscStep.
+      
+      apply oneStepClosure_grow; gen1'.
+
+
+      simplify
+      ; repeat tidy'
+      ; tidy
+      ; rstep
+      ; istep
+      ; subst
+      ; canonicalize users.
+
+      clear H1; close.
+      clear H1; close.
+      
+      ; repeat close.
+
+      simpl in H2; split_ex; subst.
+      invert H2.
+      invert H8.
+
+      (* unfold summarize_univ in H1. *)
+      (* autounfold in H1; simpl in H1. *)
+      (* specialize (H1 0); *)
+      (*   rewrite !add_neq_o in H1 by congruence; *)
+      (*   rewrite !add_eq_o in H1 by trivial; simpl in H1. *)
+      (* specialize (H1 _ {| sending_to := { } |} eq_refl); simpl in H1. *)
+
+
+      match goal with
+      | [ H : (forall _ _, ~ indexedRealStep ?uid _ ?ru _)
+            \/ (exists _ _, ?uid <> _ /\ _ $? _ = Some _ /\ (forall _, ?sums $? _ = Some _ -> commutes ?proto _ -> False))
+        , S : summarize_univ ?ru ?sums
+          |- _ ] =>
+        ( (assert (exists lbl ru', indexedRealStep uid lbl ru ru') by solve_indexedRealStep )
+        ; (assert (exists uid2 ud2, uid <> uid2
+                               /\ ru.(RealWorld.users) $? uid2 = Some ud2
+                               /\ (forall s, summaries $? uid2 = Some s -> commutes proto s)) by non_commuters ))
+        ; discharge_nextStep2 (* clear this goal since the preconditions weren't satisfied *)
+      end.
+
+      admit.
+      admit.
+      
+
+
+
+      repeat 
+      match goal with
+      end.
+        
+      specialize (H1 _ _ {| sending_to := { } |} H6); split_ex.
+      specialize (H7 _ H1); simpl in H7; contradiction.
+      
+      match goal with
+      | [ H : (forall _ _, ~ indexedRealStep ?uid _ ?ru _), ARG : indexedRealStep ?uid _ ?ru _ |- _ ] =>
+        eapply H in ARG; contradiction
+      | [ H : (forall _, ?sums $? _ = Some _ -> commutes ?proto _ -> False),
+        ARG : (forall _, ?sums $? _ = Some _ -> commutes ?proto _) |- _ ] =>
+        eapply H in ARG
+      end.
+      
+      (* specialize (H1 0); *)
+      (*   autounfold in H1; *)
+      (*   simpl in H1; *)
+      (*   rewrite !add_neq_o in H1 by congruence; *)
+      (*   rewrite !add_eq_o in H1 by trivial; *)
+      (*   specialize (H1 _ {| sending_to := { } |} eq_refl); *)
+      (*   simpl in H1; *)
+      (*   split_ex. *)
+
+      exists 0; eexists; repeat simple apply conj; [
+        congruence
+      | solve [ autounfold; simpl; clean_map_lookups; trivial ]
+      | intros; simpl
+      ]; match goal with
+         | [ |- False ] => idtac 1
+         end.
+
+      | intros; invert_commutes ].
+
+      exists 0; eexists; repeat simple apply conj; [
+        congruence
+      | solve [ autounfold; simpl; clean_map_lookups; trivial ]
+      | intros; invert_commutes ].
+
+
+
+      simplify
+      ; tidy
+      ; rstep
+      ; istep
+      ; subst
+      ; canonicalize users
+      ; repeat close.
+      
+
+
+      
+        
+         
+      simplify
+      ; repeat tidy'
+      ; tidy
+      ; repeat tidy'
+      ; idtac "rstep start"
+      ; rstep
+      ; idtac "istep start"
+      ; istep
+      ; idtac "istep done"
+      ; subst
+      ; canonicalize users
+      ; idtac "close start"
+      ; repeat close
+      ; idtac "close done".
+
+
+
+
+  Ltac gen1' :=
+    simplify
+    ; tidy
+    ; idtac "rstep start"
+    ; rstep
+    ; idtac "istep start"
+    ; istep
+    ; idtac "istep done"
+    ; subst
+    ; canonicalize users
+    ; idtac "close start"
+    ; repeat close
+    ; idtac "close done".
+      
+      invert H0.
+      invert H1.
+      invert H.
+
+      
+      simplify; simpl_sets (sets; tidy)]
+
+
+
+
+      
       gen1.
       gen1.
       gen1.
@@ -193,7 +436,7 @@ Module ShareSecretProtocolSecure <: AutomatedSafeProtocol.
             unfold safety, alignment;
             ( split;
             [ solve_honest_actions_safe; clean_map_lookups; eauto 8
-            | simpl; split; trivial; intros; rstep; subst; solve_labels_align
+            | split; trivial; intros; rstep; subst; solve_labels_align
             ]).
       
       Unshelve.
